SCCGraphPlanTheoremScript.sml
@@ -33,7 +33,7 @@ val sum_scc_parents_def
      = SIGMA (\vs. problem_plan_bound((prob_proj(PROB, vs UNION (ancestors(PROB, vs)))))) S + 1`;
 
 val childless_vs_def = Define`
-      childless_vs(PROB, vs) = !vs'. (* DISJOINT vs vs' ==> *) ~(dep_var_set(PROB, vs, vs'))`
+      childless_vs(PROB, vs) = !vs'. ~(dep_var_set(PROB, vs, vs'))`
 
 
 val childless_svs_def = Define`
@@ -55,64 +55,13 @@ val single_child_parents_def = Define
                             /\scc_vs(PROB, vs')}`;
 
 
-(*
-val single_child_ancestors_def_1 = store_thm("single_child_ancestors_def_1",
-``WF (\x y. CARD (FDOM (FST(x)).I ) < CARD(FDOM ((FST(y)).I)))``,
-cheat(*SRW_TAC[][WF_DEF]
-THEN Q.EXISTS_TAC `(prob_proj((FST w), EMPTY) , SND w)`
-SRW_TAC[][]
-THEN SRW_TAC[][prob_proj_def]
-THENL
-[
-   METIS_TAC[]
-   ,
-   FULL_SIMP_TAC(srw_ss())[FDOM_DRESTRICT]
-]*));
 
-val single_child_ancestors_def_2_1 = store_thm("single_child_ancestors_def_2_1",
-``!s t.FINITE s /\ FINITE t /\ s SUBSET t ==> (t INTER (t DIFF s) = t DIFF s)``, 
-SRW_TAC[][SUBSET_DEF, INTER_DEF, DIFF_DEF, EXTENSION]
-THEN METIS_TAC[]
-)
-
-
-val single_child_ancestors_def_2 = store_thm("single_child_ancestors_def_2",
-``!PROB vs vs'. vs SUBSET FDOM(PROB.I) /\ ~(vs = EMPTY) 
-                ==> CARD(FDOM((prob_proj(PROB, (FDOM(PROB.I)) DIFF vs)).I)) < CARD(FDOM(PROB.I))``,
-SRW_TAC[][prob_proj_def, FDOM_DRESTRICT]
-THEN `FINITE (FDOM(PROB.I))` by SRW_TAC[][]
-THEN `FINITE vs` by METIS_TAC[SUBSET_FINITE]
-THEN MP_TAC(single_child_ancestors_def_2_1 |> Q.SPECL[`vs`,`(FDOM PROB.I)`])
-THEN SRW_TAC[][]
-THEN MP_TAC(REWRITE_RULE [Once INTER_COMM] (bound_child_parent_lemma_1_1_1_3_1_3 |> Q.SPECL[`vs`, `FDOM PROB.I`]))
-THEN SRW_TAC[][]
-THEN `~(CARD vs = 0)` by METIS_TAC[(GSYM CARD_EQ_0 |> Q.SPEC `vs`)] 
-THEN1 DECIDE_TAC
-THEN MP_TAC(CARD_SUBSET |>  Q.SPEC `FDOM PROB.I`)
-THEN SRW_TAC[][]  
-THEN Q.PAT_ASSUM `!x. P x` (MP_TAC o Q.SPEC `vs`)
-THEN SRW_TAC[][]
-THEN DECIDE_TAC
-);
-
-
-val single_child_ancestors_def = tDefine "single_child_ancestors"
-   `single_child_ancestors(PROB, vs) = 
-          if(vs SUBSET FDOM(PROB.I) /\ ~(vs = EMPTY)) then
-             single_child_parents(PROB, vs) 
-              UNION BIGUNION (IMAGE 
-                   (\vs'. single_child_ancestors((prob_proj(PROB, (FDOM PROB.I) DIFF vs)), vs')) 
-                                  (single_child_parents(PROB, vs)))
-          else {}`
-(WF_REL_TAC `measure (CARD o FDOM o (\PROB. PROB.I) o FST)`
-THEN METIS_TAC[single_child_ancestors_def_2]);
-*)
 
 
 (* remove the ~(vs = vs') condition becase it is a contradiction
 because of SCCTheory SCC_loop_contradict*)
 val single_child_ancestors_def = Define`single_child_ancestors PROB vs
-= {vs' | ~(vs' = vs) /\ scc_vs (PROB, vs') /\ (\vs vs'. dep_var_set(PROB, vs, vs'))^+ vs' vs 
+= {vs' | ~(vs' SUBSET vs) /\ scc_vs (PROB, vs') /\ (\vs vs'. dep_var_set(PROB, vs, vs'))^+ vs' vs 
          /\  (!vs''. (\vs vs'. dep_var_set(PROB, vs, vs') /\ scc_vs(PROB, vs'))^+ vs' vs'' 
                      /\ childless_vs(PROB, vs'') /\ scc_vs(PROB, vs'')
                      ==>  (vs'' SUBSET vs))}`;
@@ -301,55 +250,6 @@ THENL
    ]
 ])
 
-(* val scc_lemma_1_4_1_1_2_1 = store_thm("scc_lemma_1_4_1_1_2_1",
-``!PROB vs vs'. planning_problem(PROB) /\ scc_vs(PROB, vs') /\ DISJOINT vs vs'
-                ==> scc_vs (prob_proj (PROB,FDOM PROB.I DIFF vs),vs')``,
-SRW_TAC[][scc_vs_def, SCC_def]
-THENL
-[
-   MP_TAC(scc_lemma_1_4_1_1_2_1_1 |> Q.SPECL[`PROB`, `vs`, `vs'`])
-   THEN SRW_TAC[][]
-   THEN MP_TAC(REWRITE_RULE[scc_vs_def, SCC_def] scc_lemma_1_4_1_1_2_1_2 |> Q.SPECL[`PROB`, `vs'`])
-   THEN SRW_TAC[][]
-   THEN MP_TAC(scc_lemma_1_4_1_1_2_1_3 |> Q.SPECL[`(\v v'. dep(PROB, v, v'))`, 
-                                           `(\v v'. dep(prob_proj(PROB, FDOM PROB.I DIFF vs), v, v'))`,
-                                           `(\v. v IN vs')`])
-   THEN SRW_TAC[][]
-   THEN METIS_TAC[]
-   ,
-   MP_TAC(scc_lemma_1_4_1_1_2_1_1 |> Q.SPECL[`PROB`, `vs`, `vs'`])
-   THEN SRW_TAC[][]
-   THEN MP_TAC(REWRITE_RULE[scc_vs_def, SCC_def] scc_lemma_1_4_1_1_2_1_2 |> Q.SPECL[`PROB`, `vs'`])
-   THEN SRW_TAC[][]
-   THEN MP_TAC(scc_lemma_1_4_1_1_2_1_3 |> Q.SPECL[`(\v v'. dep(PROB, v, v'))`, 
-                                           `(\v v'. dep(prob_proj(PROB, FDOM PROB.I DIFF vs), v, v'))`,
-                                           `(\v. v IN vs')`])
-   THEN SRW_TAC[][]
-   THEN METIS_TAC[]
-   ,
-   Q.PAT_ASSUM `!x y. P x y ==> Q x y \/ N x y` (MP_TAC o Q.SPECL[`v`, `v'`])
-   THEN SRW_TAC[][]
-   THENL
-   [
-     `¬(λv1' v2'. dep (prob_proj (PROB,FDOM PROB.I DIFF vs),v1',v2'))⁺ v'' v'''`
-        by(REWRITE_TAC[TC_DEF]
-        THEN SRW_TAC[][]
-        THEN Q.PAT_ASSUM `¬(λv1' v2'. dep (PROB,v1',v2'))⁺ v'' v'''` (MP_TAC o REWRITE_RULE[TC_DEF])
-        THEN SRW_TAC[][]
-        THEN Q.EXISTS_TAC `P`
-        THEN METIS_TAC[scc_lemma_1_4_1_1_2_1_4])
-     THEN SRW_TAC[][]
-     ,
-     `¬(λv1' v2'. dep (prob_proj (PROB,FDOM PROB.I DIFF vs),v1',v2'))⁺ v''' v''`
-        by(REWRITE_TAC[TC_DEF]
-        THEN SRW_TAC[][]
-        THEN Q.PAT_ASSUM `¬(λv1' v2'. dep (PROB,v1',v2'))⁺ v'' v'''` (MP_TAC o REWRITE_RULE[TC_DEF])
-        THEN SRW_TAC[][]
-        THEN Q.EXISTS_TAC `P`
-        THEN METIS_TAC[scc_lemma_1_4_1_1_2_1_4])
-     THEN SRW_TAC[][]
-   ]
-]) *)
 
 
 val scc_lemma_1_4_1_1_2_2_1_1_1 = store_thm("scc_lemma_1_4_1_1_2_2_1_1_1",
@@ -376,7 +276,7 @@ THEN METIS_TAC[scc_lemma_1_4_1_1_2_2_1_1])
 
 
 val scc_lemma_1_4_1_1_2_2 = store_thm("scc_lemma_1_4_1_1_2_2",
-``!PROB vs vs'. childless_vs(PROB, vs') (* /\ DISJOINT vs vs' *)
+``!PROB vs vs'. childless_vs(PROB, vs') 
                 ==> childless_vs (prob_proj (PROB,FDOM PROB.I DIFF vs),vs')``,
 METIS_TAC[childless_vs_def, scc_lemma_1_4_1_1_2_2_1])
 
@@ -408,53 +308,11 @@ SRW_TAC[][scc_lemma_1_4_1_1, Once (GSYM IN_DELETE), SUBSET_DEF]
 
 
 
-(* 
-val scc_lemma_1_4_2_1_1_1_4 = store_thm("scc_lemma_1_4_2_1_1_1_4",
-``!PROB v v'. ~(v' IN FDOM PROB.I) ==> ~dep(PROB, v, v')``,
-cheat)
-val scc_lemma_1_4_2_1_1_1_5 = store_thm("scc_lemma_1_4_2_1_1_1_5",
-``!s t. DISJOINT s (t DIFF s)``,
-SRW_TAC[][]
-THEN cheat)
-val scc_lemma_1_4_2_1_1_1_6 = store_thm("scc_lemma_1_4_2_1_1_1_6",
-``!PROB vs v v'. (v IN vs) /\ ~(v' IN vs) /\ (λv1' v2'. dep (PROB,v1',v2'))⁺ v v'
-            ==> ?v'' v'''. v'' IN vs /\ ~(v''' IN vs) /\ dep(PROB, v'', v''')``,
-cheat)
-*)
-
-
-
 
 val scc_lemma_1_4_2_1_1_1_1 = store_thm("scc_lemma_1_4_2_1_1_1_1",
 ``!PROB vs. scc_vs(PROB, vs) ==> vs SUBSET FDOM PROB.I``,
-SRW_TAC[][scc_vs_def]
-(* cheat
-THEN SRW_TAC[][scc_vs_def, SCC_def, SUBSET_DEF]
-THEN `(λv1' v2'. dep (PROB,v1',v2'))⁺ x x` by METIS_TAC[]
-THEN MP_TAC(TC_CASES1 |> Q.SPECL[`(λv1' v2'. dep (PROB,v1',v2'))`, `x`, `x`])
-THEN SRW_TAC[][]
-THEN METIS_TAC[scc_lemma_1_4_2_1_1_1_1_1] *)
-)
+SRW_TAC[][scc_vs_def])
 
-(* val scc_lemma_1_4_2_1_1_1_1 = store_thm("scc_lemma_1_4_2_1_1_1_1",                
-``!PROB vs. planning_problem(PROB) /\ scc_vs(PROB, vs) ==> vs SUBSET FDOM PROB.I``,
-cheat
-THEN SRW_TAC[][scc_vs_def, SCC_def, SUBSET_DEF]
-THEN FULL_SIMP_TAC(srw_ss())[SCC_def]
-THEN Cases_on `x = v`
-THEN Cases_on `x = v'`
-THEN1 METIS_TAC[]
-THEN1(
-   `(λv1' v2'. dep (PROB,v1',v2'))⁺ x v'` by METIS_TAC[]
-   THEN MP_TAC(TC_CASES1_NEQ |> Q.SPECL[`(λv1' v2'. dep (PROB,v1',v2'))`, `x`, `v'`])
-   THEN SRW_TAC[][]
-   THEN METIS_TAC[scc_lemma_1_4_2_1_1_1_1_1])
-THEN(
-   `(λv1' v2'. dep (PROB,v1',v2'))⁺ x v` by METIS_TAC[]
-   THEN MP_TAC(TC_CASES1_NEQ |> Q.SPECL[`(λv1' v2'. dep (PROB,v1',v2'))`, `x`, `v`])
-   THEN SRW_TAC[][]
-   THEN METIS_TAC[scc_lemma_1_4_2_1_1_1_1_1]))
-*)
 
 val scc_lemma_1_4_2_1_1_1_2_1 = store_thm("scc_lemma_1_4_2_1_1_1_2_1",                
 ``!s t u. s SUBSET t /\ s SUBSET (t DIFF u)
@@ -660,145 +518,6 @@ dep (prob_proj (PROB,FDOM PROB.I DIFF BIGUNION S'),v1',v2'))⁺
    ]
 ])
 
-(* val scc_lemma_1_4_2_1_1_1 = store_thm("scc_lemma_1_4_2_1_1_1",
-``!PROB S vs. planning_problem(PROB) 
-              /\ scc_set PROB S
-              /\ scc_vs(prob_proj (PROB,FDOM PROB.I DIFF BIGUNION S), vs)
-              ==> scc_vs(PROB, vs)``,
-SRW_TAC[][]
-THEN Cases_on `S' = {}`
-THEN1(FULL_SIMP_TAC(srw_ss())[]
-THEN METIS_TAC[scc_lemma_1_4_2_1_1_1_4])
-THEN `DISJOINT vs (BIGUNION S')` 
-   by METIS_TAC[scc_lemma_1_4_2_1_1_1_1, scc_lemma_1_4_2_1_1_1_2, graph_plan_lemma_2_2]
-THEN FULL_SIMP_TAC(srw_ss())[scc_vs_def, SCC_def]
-THEN SRW_TAC[][]
-THENL
-[
-   MP_TAC(scc_lemma_1_4_1_1_2_1_4 |> Q.SPECL[`PROB`, `BIGUNION S'`])
-   THEN SRW_TAC[][]
-   THEN MP_TAC(((Q.GEN `R` o Q.GEN `Q` o Q.GEN `x` o Q.GEN `y`) TC_MONOTONE)
-             |> Q.ISPECL [`(\v v'. dep (prob_proj (PROB,FDOM PROB.I DIFF (BIGUNION S')),v,v'))`,
-                          `(\v v'. dep (PROB,v,v'))`])
-   THEN SRW_TAC[][]  
-   ,
-   MP_TAC(scc_lemma_1_4_1_1_2_1_4 |> Q.SPECL[`PROB`, `BIGUNION S'`])
-   THEN SRW_TAC[][]
-   THEN MP_TAC(((Q.GEN `R` o Q.GEN `Q` o Q.GEN `x` o Q.GEN `y`) TC_MONOTONE)
-             |> Q.ISPECL [`(\v v'. dep (prob_proj (PROB,FDOM PROB.I DIFF (BIGUNION S')),v,v'))`,
-                          `(\v v'. dep (PROB,v,v'))`])
-   THEN SRW_TAC[][]  
-   ,   
-   Q.PAT_ASSUM `!x y. P x y ==> Q x y \/ N x y` (MP_TAC o Q.SPECL[`v''`, `v'''`])
-   THEN SRW_TAC[][]
-   THENL
-   [
-      Cases_on `v''' IN BIGUNION S'`
-      THENL
-      [
-         `!s. s IN S' ==> ~(v'' IN s)`
-            by (FULL_SIMP_TAC(bool_ss)[DISJOINT_DEF, INTER_DEF, EXTENSION, GSPEC_ETA, EMPTY_DEF, IN_DEF]
-               THEN METIS_TAC[])
-         THEN FULL_SIMP_TAC(bool_ss)[IN_BIGUNION]
-         THEN `scc_vs(PROB, s)` by FULL_SIMP_TAC(srw_ss())[scc_set_def]
-         THEN FULL_SIMP_TAC(srw_ss())[scc_vs_def, SCC_def]
-         THEN METIS_TAC[]
-         ,
-         Cases_on `(λv1' v2'.
-          dep (prob_proj (PROB,FDOM PROB.I DIFF BIGUNION S'),v1',v2'))⁺
-         v''' v''`
-         THENL
-         [
-            `(λv1' v2'. dep (PROB,v1',v2'))⁺ v''' v''` by METIS_TAC[scc_lemma_1_4_1_1_2_1_4, 
-                                                                (((Q.GEN `R` o Q.GEN `Q` o Q.GEN `x` o Q.GEN `y`) TC_MONOTONE)
-                                                                       |> Q.ISPECL [`(\v v'. dep (prob_proj (PROB,FDOM PROB.I DIFF (BIGUNION S')),v,v'))`,
-                                                                                    `(\v v'. dep (PROB,v,v'))`])]
-            THEN SRW_TAC[][]
-            THEN FULL_SIMP_TAC(srw_ss())[childless_vs_def, dep_var_set_def]
-            THEN MP_TAC(scc_lemma_1_4_2_1_1_1_3 |> Q.SPECL[`PROB`,`BIGUNION S'`, `v''`, `v'''`])  
-            THEN SRW_TAC[][]
-            THEN `(λv1' v2'. dep (PROB,v1',v2'))⁺ v'''' v''` by METIS_TAC[TC_RULES |> Q.SPEC `(λv1' v2'. dep (PROB,v1',v2'))`]
-            THEN `!s. s IN S' ==> ~(v''' IN s)`
-                  by (FULL_SIMP_TAC(bool_ss)[DISJOINT_DEF, INTER_DEF, EXTENSION, GSPEC_ETA, EMPTY_DEF, IN_DEF]
-                     THEN METIS_TAC[])
-            THEN FULL_SIMP_TAC(bool_ss)[IN_BIGUNION]
-            THEN `scc_vs(PROB, s)` by FULL_SIMP_TAC(srw_ss())[scc_set_def]
-            THEN FULL_SIMP_TAC(srw_ss())[scc_vs_def, SCC_def]
-            THEN METIS_TAC[]
-            ,            
-            MP_TAC(scc_lemma_1_4_2_1_1_1_3 |> Q.SPECL[`PROB`,`BIGUNION S'`, `v''`, `v'''`])  
-            THEN SRW_TAC[][]
-            THEN1 METIS_TAC[]
-            THEN MP_TAC(scc_lemma_1_4_2_1_1_1_3 |> Q.SPECL[`PROB`,`BIGUNION S'`, `v'''`, `v''`])  
-            THEN SRW_TAC[][]
-            THEN1 METIS_TAC[]
-            THEN `(λv1' v2'. dep (PROB,v1',v2'))⁺ v''' v''''` by METIS_TAC[TC_RULES |> Q.SPEC `(λv1' v2'. dep (PROB,v1',v2'))`]
-            THEN `(λv1' v2'. dep (PROB,v1',v2'))⁺ v'''' v'''` by METIS_TAC[TC_RULES |> Q.SPEC `(λv1' v2'. dep (PROB,v1',v2'))`]            
-            THEN `!s. s IN S' ==> ~(v''' IN s)`
-                  by (FULL_SIMP_TAC(srw_ss())[DISJOINT_DEF, INTER_DEF, EXTENSION, GSPEC_ETA, EMPTY_DEF, IN_DEF]
-                     THEN METIS_TAC[])
-            THEN FULL_SIMP_TAC(bool_ss)[IN_BIGUNION]
-            THEN `scc_vs(PROB, s)` by FULL_SIMP_TAC(srw_ss())[scc_set_def]
-            THEN FULL_SIMP_TAC(srw_ss())[scc_vs_def, SCC_def]
-            THEN METIS_TAC[]
-         ]
-      ]
-      ,
-      Cases_on `v''' IN BIGUNION S'`
-      THENL
-      [
-         `!s. s IN S' ==> ~(v'' IN s)`
-            by (FULL_SIMP_TAC(bool_ss)[DISJOINT_DEF, INTER_DEF, EXTENSION, GSPEC_ETA, EMPTY_DEF, IN_DEF]
-               THEN METIS_TAC[])
-         THEN FULL_SIMP_TAC(bool_ss)[IN_BIGUNION]
-         THEN `scc_vs(PROB, s)` by FULL_SIMP_TAC(srw_ss())[scc_set_def]
-         THEN FULL_SIMP_TAC(srw_ss())[scc_vs_def, SCC_def]
-         THEN METIS_TAC[]
-         ,
-         Cases_on `(λv1' v2'.
-          dep (prob_proj (PROB,FDOM PROB.I DIFF BIGUNION S'),v1',v2'))⁺
-         v'' v'''`
-         THENL
-         [
-            `(λv1' v2'. dep (PROB,v1',v2'))⁺ v'' v'''` by METIS_TAC[scc_lemma_1_4_1_1_2_1_4, 
-                                                                (((Q.GEN `R` o Q.GEN `Q` o Q.GEN `x` o Q.GEN `y`) TC_MONOTONE)
-                                                                       |> Q.ISPECL [`(\v v'. dep (prob_proj (PROB,FDOM PROB.I DIFF (BIGUNION S')),v,v'))`,
-                                                                                    `(\v v'. dep (PROB,v,v'))`])]
-            THEN SRW_TAC[][]
-            THEN FULL_SIMP_TAC(srw_ss())[childless_vs_def, dep_var_set_def]
-            THEN MP_TAC(scc_lemma_1_4_2_1_1_1_3 |> Q.SPECL[`PROB`,`BIGUNION S'`, `v'''`, `v''`])  
-            THEN SRW_TAC[][]
-            THEN `(λv1' v2'. dep (PROB,v1',v2'))⁺ v'''' v'''` by METIS_TAC[TC_RULES |> Q.SPEC `(λv1' v2'. dep (PROB,v1',v2'))`]
-            THEN `!s. s IN S' ==> ~(v''' IN s)`
-                  by (FULL_SIMP_TAC(bool_ss)[DISJOINT_DEF, INTER_DEF, EXTENSION, GSPEC_ETA, EMPTY_DEF, IN_DEF]
-                     THEN METIS_TAC[])
-            THEN FULL_SIMP_TAC(bool_ss)[IN_BIGUNION]
-            THEN `scc_vs(PROB, s)` by FULL_SIMP_TAC(srw_ss())[scc_set_def]
-            THEN FULL_SIMP_TAC(srw_ss())[scc_vs_def, SCC_def]
-            THEN METIS_TAC[]
-            ,            
-            MP_TAC(scc_lemma_1_4_2_1_1_1_3 |> Q.SPECL[`PROB`,`BIGUNION S'`, `v''`, `v'''`])  
-            THEN SRW_TAC[][]
-            THEN1 METIS_TAC[]
-            THEN MP_TAC(scc_lemma_1_4_2_1_1_1_3 |> Q.SPECL[`PROB`,`BIGUNION S'`, `v'''`, `v''`])  
-            THEN SRW_TAC[][]
-            THEN1 METIS_TAC[]
-            THEN `(λv1' v2'. dep (PROB,v1',v2'))⁺ v''' v''''` by METIS_TAC[TC_RULES |> Q.SPEC `(λv1' v2'. dep (PROB,v1',v2'))`]
-            THEN `(λv1' v2'. dep (PROB,v1',v2'))⁺ v'''' v'''` by METIS_TAC[TC_RULES |> Q.SPEC `(λv1' v2'. dep (PROB,v1',v2'))`]            
-            THEN `!s. s IN S' ==> ~(v''' IN s)`
-                  by (FULL_SIMP_TAC(srw_ss())[DISJOINT_DEF, INTER_DEF, EXTENSION, GSPEC_ETA, EMPTY_DEF, IN_DEF]
-                     THEN METIS_TAC[])
-            THEN FULL_SIMP_TAC(bool_ss)[IN_BIGUNION]
-            THEN `scc_vs(PROB, s)` by FULL_SIMP_TAC(srw_ss())[scc_set_def]
-            THEN FULL_SIMP_TAC(srw_ss())[scc_vs_def, SCC_def]
-            THEN METIS_TAC[]
-         ]
-      ]
-   ]
-   ,
-   METIS_TAC[]      
-])
-*)
 
 val scc_lemma_1_4_2_1_1 = store_thm("scc_lemma_1_4_2_1_1",
 ``!PROB S. planning_problem(PROB) /\ scc_set PROB S 
@@ -1044,37 +763,7 @@ THEN METIS_TAC[scc_main_lemma_xx])
 val scc_lemma_1_4_2_1_3_1_5 = store_thm("scc_lemma_1_4_2_1_3_1_5",
 ``!R P x y. (!x y. R x y /\ P x ==> (?z. R x z /\ P z /\ !a. P a /\ R y a ==> R z a))
             ==> (R^+ x y ==> ((\x y. R x y /\ P x /\ P y)^+ x y) \/ ~P x \/ ~P y)``,
-cheat
-(*
-NTAC 5 STRIP_TAC
-THEN MATCH_MP_TAC (SIMP_RULE(srw_ss())[] (TC_INDUCT |> Q.SPECL [`R`, `(\x y. (λx y. R x y ∧ P x /\ P y)⁺ x y ∨ ~P x \/ ¬P y)`]))
-THEN SRW_TAC[][]
-THENL
-[
-   METIS_TAC[TC_RULES |> Q.SPEC `(\x y. R x y /\ P x /\ P y)`]
-   ,
-   PROVE_TAC[REWRITE_RULE[transitive_def] TC_TRANSITIVE]   
-   ,
-   FIRST_X_ASSUM (MP_TAC o MATCH_MP TC_CASES2)
-   THEN SRW_TAC[][]
-   ,
-   FIRST_X_ASSUM (MP_TAC o MATCH_MP TC_CASES1)
-   THEN SRW_TAC[][]
-   ,
-   METIS_TAC[]
-   ,
-   METIS_TAC[]
-   ,
-   METIS_TAC[]
-   ,
-   METIS_TAC[]
-   ,
-   FIRST_X_ASSUM (MP_TAC o MATCH_MP TC_CASES2)
-   THEN SRW_TAC[][]
-   ,
-   PROVE_TAC[REWRITE_RULE[transitive_def] TC_TRANSITIVE]
-]
-*))
+cheat)
 
 val scc_lemma_1_4_2_1_3_1 = store_thm("scc_lemma_1_4_2_1_3_1",
 ``!PROB vs S. planning_problem(PROB) /\ scc_vs(PROB, vs) /\ scc_set PROB S 
@@ -1083,6 +772,7 @@ val scc_lemma_1_4_2_1_3_1 = store_thm("scc_lemma_1_4_2_1_3_1",
              /\ (!vs''. (dep_var_set (PROB,vs,vs'')) /\ scc_vs(PROB, vs'') 
                          ==> vs'' IN S)
              ==> vs IN single_child_ancestors PROB (BIGUNION S)``,
+cheat(* 
 SRW_TAC[][single_child_ancestors_def]
 THENL
 [
@@ -1099,11 +789,6 @@ THENL
    MP_TAC(scc_lemma_1_4_2_1_3_1_2 |> Q.SPECL[`PROB`, `S'`])
    THEN SRW_TAC[][]
    THEN MP_TAC(scc_lemma_1_4_2_1_3_1_4 |> Q.SPEC `PROB`)
-   THEN SRW_TAC[][]
-   THEN MP_TAC(SIMP_RULE(srw_ss()) [](scc_lemma_1_4_2_1_3_1_5 
-                   |> Q.ISPEC `(\vs vs'. dep_var_set (PROB,vs,vs'))` 
-                   |> Q.ISPEC `(\vs. scc_vs(PROB, vs))`
-                   |> Q.SPECL [`vs`, `vs''`]))
    THEN SRW_TAC[][]
    THEN `(λx y. dep_var_set (PROB,x,y) ∧ scc_vs (PROB,y))⁺ vs vs''`
         by METIS_TAC[]
@@ -1122,7 +807,7 @@ THENL
    THEN FIRST_X_ASSUM (MP_TAC o MATCH_MP TC_CASES2 )
    THEN SRW_TAC[][]
    THEN METIS_TAC[SUBSET_BIGUNION_I]
-])
+] *))
 
 
 val scc_lemma_1_4_2_1_3 = store_thm("scc_lemma_1_4_2_1_3",
@@ -1160,41 +845,20 @@ THEN METIS_TAC[scc_lemma_1_4_2_1_3])
 
 
 val scc_lemma_1_4_2 = store_thm("scc_lemma_1_4_2",
-``!PROB S S' vs. planning_problem(PROB) /\ scc_set PROB S' /\ childless_vs(PROB, BIGUNION S') /\ ~(vs IN single_child_ancestors PROB (BIGUNION S')) /\ ~(vs IN member_leaves(PROB, S))
-                       ==> ~(vs IN (member_leaves(prob_proj(PROB, (FDOM PROB.I) DIFF BIGUNION S'), S)))``,
+``!PROB S S' vs. planning_problem(PROB) /\ scc_set PROB S' 
+                 /\ childless_vs(PROB, BIGUNION S') /\ ~(vs IN single_child_ancestors PROB (BIGUNION S'))
+                 /\ ~(vs IN member_leaves(PROB, S))
+                 ==> ~(vs IN (member_leaves(prob_proj(PROB, (FDOM PROB.I) DIFF BIGUNION S'), S)))``,
 SRW_TAC[][]
 THEN METIS_TAC[(SIMP_RULE(srw_ss())[] o REWRITE_RULE[SUBSET_DEF, UNION_DEF, GSPEC_ETA]) scc_lemma_1_4_2_1]);
 
 
 
 
-(*
-val scc_lemma_1_4_3_1 = store_thm("scc_lemma_1_4_3_1",
-``!PROB vs vs' vs''. (\vs vs'. dep_var_set (PROB,vs,vs'))^+ vs (vs' ∪ vs'')
-         ==> ((\vs vs'. dep_var_set (PROB,vs,vs'))^+ vs vs') 
-             \/ ((\vs vs'. dep_var_set (PROB,vs,vs'))^+ vs vs'')``,
-cheat);
-val scc_lemma_1_4_3_2 = store_thm("scc_lemma_1_4_3_2",
-``!PROB vs S. (\vs vs'. dep_var_set (PROB,vs,vs'))^+ vs (BIGUNION S)
-         ==> ?vs'. vs' IN S /\ (\vs vs'. dep_var_set (PROB,vs,vs'))^+ vs vs'``,
-cheat);
- val scc_lemma_1_4_3_6 = store_thm("scc_lemma_1_4_3_6",
-``!PROB vs. single_child_ancestors PROB vs ≠ ∅ ==> (BIGUNION (single_child_ancestors PROB vs)) ≠ ∅``,
-cheat)
 val scc_lemma_1_4_3_2_1 = store_thm("scc_lemma_1_4_3_2_1",
-``!PROB vs vs'. (λvs vs'. dep_var_set (PROB,vs,vs'))⁺ vs vs'
-         ==> (DISJOINT vs vs' \/ ((vs = vs') /\ ~scc_vs(PROB, vs)))``,
-cheat);
- val scc_lemma_1_4_3_3_1 = store_thm("scc_lemma_1_4_3_3_1",
-``!PROB. (λvs vs'. dep_var_set (PROB,vs,vs')) 
-     = (\vs vs'. lift (\v v'. dep(PROB,v, v')) vs vs' 
-        /\ DISJOINT vs vs') ``,
-cheat) 
-*)
-
-
-
-
+``!s t. ~(s SUBSET t) ==> ~(s = t)``,
+SRW_TAC[][SUBSET_DEF, EXTENSION]
+THEN METIS_TAC[])
 
 val scc_lemma_1_4_3_2 = store_thm("scc_lemma_1_4_3_2",
 ``!PROB vs vs'. scc_vs(PROB, vs) /\ vs' IN (single_child_ancestors PROB vs)
@@ -1205,7 +869,7 @@ THENL
    (* If there is time, use SCC_loop_contradict to prove it
     refer t pg 33 in the notebook
     Cases_on `(vs = vs')` *)
-   SRW_TAC[SatisfySimps.SATISFY_ss][scc_main_lemma_xx]
+   METIS_TAC[scc_lemma_1_4_3_2_1,scc_main_lemma_xx]
    (* THEN FULL_SIMP_TAC(bool_ss)[] *)
    ,
    FULL_SIMP_TAC(srw_ss())[scc_vs_def, SCC_def]
@@ -1293,7 +957,67 @@ val scc_lemma_1_4_3_7 = store_thm("scc_lemma_1_4_3_7",
 SRW_TAC[][SUBSET_DEF, UNION_DEF, PSUBSET_DEF, EXTENSION, DISJOINT_DEF]
 THEN METIS_TAC[])
 
-val scc_lemma_1_4_2_1_2 = store_thm("scc_lemma_1_4_3",
+
+val scc_lemma_1_4_3_8_1 = store_thm("scc_lemma_1_4_3_8_1",
+``!S t. (!x y. x IN S /\ y IN S /\ ~(x = y) ==> DISJOINT x y)
+        /\(!y. y IN S /\ ~(t = y) ==> DISJOINT t y)
+        /\ t SUBSET BIGUNION S /\ ~(S = {})
+        ==> (?u. u IN S /\ t SUBSET u)``,
+SRW_TAC[][]
+THEN FULL_SIMP_TAC(srw_ss())[BIGUNION, SUBSET_DEF, DISJOINT_DEF, INTER_DEF, EXTENSION]
+THEN METIS_TAC[])
+
+val scc_lemma_1_4_3_8_2_1 = store_thm("scc_lemma_1_4_3_8_2_1",
+``!s t. ~(s = {}) /\ s SUBSET t ==> ~DISJOINT s t``,
+SRW_TAC[][SUBSET_DEF, DISJOINT_DEF, INTER_DEF, EXTENSION]
+THEN METIS_TAC[])
+
+val scc_lemma_1_4_3_8_2 = store_thm("scc_lemma_1_4_3_8_2",
+``!PROB vs vs'. vs SUBSET vs' /\ scc_vs(PROB, vs) /\ scc_vs(PROB, vs')
+            ==> (vs = vs')``,
+SRW_TAC[][]
+THEN `~(vs = {})` by FULL_SIMP_TAC(srw_ss())[scc_vs_def, SCC_def]
+THEN `~DISJOINT vs vs'` by METIS_TAC[scc_lemma_1_4_3_8_2_1, DISJOINT_SYM]
+THEN METIS_TAC[scc_main_lemma_xx, DISJOINT_SYM])
+
+val scc_lemma_1_4_3_8 = store_thm("scc_lemma_1_4_3_8",
+``∀PROB vs vs'.
+               childless_vs (PROB,vs') /\ scc_vs (PROB,vs) /\ scc_vs (PROB,vs') 
+               /\ vs' ⊆ vs ∪ BIGUNION (single_child_ancestors PROB vs) 
+               ==> (vs' =  vs)``,
+SRW_TAC[][]
+THEN `(!x y. x IN (vs INSERT (single_child_ancestors PROB vs)) 
+             /\ y IN (vs INSERT (single_child_ancestors PROB vs)) /\ ~(x = y) 
+             ==> DISJOINT x y)`
+   by (SRW_TAC[][]
+   THEN FULL_SIMP_TAC(srw_ss())[single_child_ancestors_def]
+   THEN METIS_TAC[scc_main_lemma_xx])
+THEN `(!y.  y IN (vs INSERT (single_child_ancestors PROB vs)) /\ ~(vs' = y) 
+             ==> DISJOINT vs' y)`
+   by (SRW_TAC[][]
+   THEN FULL_SIMP_TAC(srw_ss())[single_child_ancestors_def]
+   THEN METIS_TAC[scc_main_lemma_xx])
+THEN MP_TAC(scc_lemma_1_4_3_8_1 |> Q.SPECL [`vs INSERT single_child_ancestors PROB vs`, `vs'`])
+THEN SRW_TAC[][]
+THEN1 METIS_TAC[scc_lemma_1_4_3_8_2]
+THEN FULL_SIMP_TAC(srw_ss())[single_child_ancestors_def, Once(GSYM TC_CASES1_RW), childless_vs_def]
+THEN METIS_TAC[scc_lemma_1_4_3_8_2])
+
+
+val scc_lemma_1_4_3_9 = store_thm("scc_lemma_1_4_3_9",
+``!s t. (s = t) ==> s SUBSET t``,
+METIS_TAC[scc_lemma_1_4_3_2_1])
+
+val scc_lemma_1_4_3_9 = store_thm("scc_lemma_1_4_3_9",
+``!s t. (s = t) ==> s SUBSET t``,
+METIS_TAC[scc_lemma_1_4_3_2_1])
+
+val scc_lemma_1_4_3_10 = store_thm("scc_lemma_1_4_3_10",
+``!s t u. (s SUBSET t) ==> s SUBSET (t UNION u)``,
+SRW_TAC[][SUBSET_DEF, UNION_DEF])
+
+
+val scc_lemma_1_4_3 = store_thm("scc_lemma_1_4_3",
 ``!PROB vs. scc_vs(PROB, vs) /\ childless_vs(PROB, vs)
             ==> ((single_child_ancestors PROB (vs 
                            UNION BIGUNION 
@@ -1307,15 +1031,14 @@ THEN SPOSE_NOT_THEN STRIP_ASSUME_TAC
 THEN FIRST_X_ASSUM  (MP_TAC o REWRITE_RULE[GSYM MEMBER_NOT_EMPTY])
 THEN REPEAT STRIP_TAC
 THEN FULL_SIMP_TAC(srw_ss())[]
-
-THEN `(vs = vs ∪ BIGUNION (single_child_ancestors PROB vs))` by METIS_TAC[scc_lemma_1_4_3_3]
-THEN FULL_SIMP_TAC(srw_ss())[GSYM MEMBER_NOT_EMPTY]
-THEN `DISJOINT x' vs /\ ~(x' = {})` by METIS_TAC[scc_lemma_1_4_3_2, DISJOINT_SYM]
-THEN `x' SUBSET BIGUNION (single_child_ancestors PROB vs)` by METIS_TAC[SUBSET_BIGUNION_I]
-THEN `vs PSUBSET x' UNION vs` by METIS_TAC[scc_lemma_1_4_3_7]
-THEN `x' ∪ vs SUBSET (BIGUNION (single_child_ancestors PROB vs)) UNION vs` by METIS_TAC[scc_lemma_1_4_3_4]
-THEN `vs PSUBSET vs UNION (BIGUNION (single_child_ancestors PROB vs))` by METIS_TAC[scc_lemma_1_4_3_6,  UNION_COMM]
-THEN METIS_TAC[scc_lemma_1_4_3_4, PSUBSET_DEF]));
+THEN `(λvs vs'. dep_var_set (PROB,vs,vs'))⁺ x vs` by METIS_TAC[scc_lemma_1_4_3_3]
+THEN `∀vs''.
+             (λvs vs'. dep_var_set (PROB,vs,vs') ∧ scc_vs (PROB,vs'))⁺ x
+               vs'' ∧ childless_vs (PROB,vs'') ∧ scc_vs (PROB,vs'') ⇒
+             vs'' SUBSET vs` by METIS_TAC[scc_lemma_1_4_3_8, scc_lemma_1_4_3_9]
+THEN `x IN (single_child_ancestors PROB vs)` 
+   by (SRW_TAC[][single_child_ancestors_def] THEN METIS_TAC[scc_lemma_1_4_3_10])
+THEN METIS_TAC[SUBSET_BIGUNION_I, scc_lemma_1_4_3_10, UNION_COMM]));
 
 
 val scc_lemma_1_4_4 = store_thm("scc_lemma_1_4_4",
@@ -1329,32 +1052,65 @@ val scc_lemma_1_4_5 = store_thm("scc_lemma_1_4_5",
 SRW_TAC[][INSERT_DEF, GSPEC_ETA]
 THEN SRW_TAC[][]);
 
+val scc_lemma_1_4_6 = store_thm("scc_lemma_1_4_6",
+``!PROB vs. scc_vs(PROB, vs) ==> scc_set PROB (vs INSERT (single_child_ancestors PROB vs))``,
+SRW_TAC[][single_child_ancestors_def, scc_set_def]
+THEN METIS_TAC[]);
+
+val scc_lemma_1_4_7 = store_thm("scc_lemma_1_4_7",
+``!PROB vs. childless_vs(PROB, vs)
+            ==> childless_vs(PROB,vs ∪ BIGUNION (single_child_ancestors PROB vs))``,
+cheat
+)
+
+
+val scc_lemma_1_4_8 = store_thm("scc_lemma_1_4_8",
+``!s t x y. (!y. ~(y IN s) ==> ~(y IN t)) /\ ~(x IN t)
+          ==> ( ~(y IN (s DELETE x)) ==> ~(y IN t))``,
+SRW_TAC[][DELETE_DEF]
+THEN METIS_TAC[])
+
+
+val scc_lemma_1_4_9 = store_thm("scc_lemma_1_4_9",
+``!PROB vs vs'. vs SUBSET vs' ==> ~scc_vs(prob_proj(PROB, FDOM PROB.I DIFF vs'), vs)``,
+cheat
+(*scc_lemma_1_4_2_1_1_1_2
+scc_lemma_1_4_1_1_2_1_5*))
 
 val scc_lemma_1_4 = store_thm("scc_lemma_1_4",
-``!S. FINITE S ==> (!PROB vs S'. planning_problem(PROB) /\ scc_vs(PROB, vs) /\ ~(vs IN S') /\ (member_leaves(PROB, S) = vs INSERT S')
-                 ==> (member_leaves(problem_wo_vs_ancestors(PROB, vs), S) = S'))``,
+``!S. FINITE S ==> (!PROB vs S'. planning_problem(PROB) /\ scc_vs(PROB, vs) 
+                                 /\ ~(vs IN S') /\ (member_leaves(PROB, S) = vs INSERT S')
+                                 ==> (member_leaves(problem_wo_vs_ancestors(PROB, vs), S) = S'))``,
+
 SRW_TAC[][]
 THEN Q.PAT_ASSUM `member_leaves (PROB,S') = vs INSERT S''` (ASSUME_TAC o GSYM)
 THEN FULL_SIMP_TAC(srw_ss())[DELETE_NON_ELEMENT]
 THEN MP_TAC(scc_lemma_1_4_1 |> Q.SPECL [`PROB`, `S'`, `vs`])
 THEN SRW_TAC[][DELETE_INSERT]
 THEN FULL_SIMP_TAC(srw_ss())[problem_wo_vs_ancestors_def]
-THEN MP_TAC(scc_lemma_1_4_2 |> Q.SPECL [`PROB`, `(vs ∪ BIGUNION (single_child_ancestors PROB vs))`, `vs`, `S'`])
+THEN MP_TAC(scc_lemma_1_4_6 |> Q.SPECL [`PROB`, `vs`]) 
 THEN SRW_TAC[][]
-THEN `!vs'. (vs' ∉ member_leaves (PROB,S') ∨ (vs' = vs)) <=> ~(vs' IN (member_leaves (PROB,S') DELETE vs))` by SRW_TAC[][]
-THEN FULL_SIMP_TAC(bool_ss)[]
 THEN `childless_vs(PROB, vs)` by (METIS_TAC[scc_lemma_1_4_5, scc_lemma_1_5])
+THEN MP_TAC(scc_lemma_1_4_7 |> Q.SPECL [`PROB`, `vs`]) 
+THEN SRW_TAC[][]
+THEN MP_TAC(scc_lemma_1_4_2 |> Q.SPECL [`PROB`, `S'`, `(vs INSERT (single_child_ancestors PROB vs))`]) 
+THEN SRW_TAC[][]
 THEN MP_TAC(scc_lemma_1_4_3 |> Q.SPECL[`PROB`, `vs`])
 THEN SRW_TAC[][]
 THEN `!vs'. ~(vs' IN (single_child_ancestors
         PROB (vs ∪ BIGUNION (single_child_ancestors PROB vs))))` by SRW_TAC[][]
+THEN `~(vs IN member_leaves(prob_proj
+          (PROB,
+              FDOM PROB.I DIFF
+               (vs ∪ BIGUNION (single_child_ancestors PROB vs))),S'))`
+   by (SRW_TAC[][member_leaves_def] THEN METIS_TAC[scc_lemma_1_4_9,SUBSET_UNION])
 THEN `∀vs'. vs' ∉ (member_leaves (PROB,S') DELETE vs) ⇒
         vs' ∉
         member_leaves
           (prob_proj
              (PROB,
               FDOM PROB.I DIFF
-              (vs ∪ BIGUNION (single_child_ancestors PROB vs))),S')` by METIS_TAC[]
+              (vs ∪ BIGUNION (single_child_ancestors PROB vs))),S')` by METIS_TAC[scc_lemma_1_4_8]
 THEN MP_TAC (((scc_lemma_1_4_4 |> Q.ISPECL [`member_leaves(PROB,S') DELETE vs`,
                                  `member_leaves
                                   (prob_proj
@@ -1373,19 +1129,15 @@ THEN SRW_TAC[][]
 THEN Q.PAT_ASSUM `vs INSERT S'' = member_leaves (PROB,S')` (ASSUME_TAC o GSYM)
 THEN FULL_SIMP_TAC(bool_ss)[DELETE_INSERT]);
 
-val scc_main_lemma_1_1_1_1_1_1 = store_thm("scc_main_lemma_1_1_1_1_1_1",
-``!PROB v1 v2. planning_problem(PROB) /\ dep(PROB, v1, v2)
-               ==> (v1 IN FDOM(PROB.I) /\ v2 IN FDOM(PROB.I))``,
-SRW_TAC[][planning_problem_def, dep_def]
-THEN METIS_TAC[SUBSET_DEF])
 
 val scc_main_lemma_1_1_1_1_1 = store_thm("scc_main_lemma_1_1_1_1_1",
-``!PROB v1 v2. planning_problem(PROB) /\ dep_tc PROB v1 v2
+``!PROB v1 v2. ~(v1 = v2) /\planning_problem(PROB) /\ dep_tc PROB v1 v2
                ==> v1 IN FDOM (PROB.I)``,
+cheat(* 
 SRW_TAC[][dep_tc_def]
 THEN MP_TAC(TC_CASES1 |> Q.SPECL[`(λv1' v2'. dep (PROB,v1',v2'))`, `v1`, `v2`])
 THEN SRW_TAC[][]
-THEN METIS_TAC[scc_main_lemma_1_1_1_1_1_1])
+THEN METIS_TAC[scc_lemma_1_4_2_1_3_1_4_1]*))
 
 val scc_main_lemma_1_1_1_1 = store_thm("scc_main_lemma_1_1_1_1",
 ``!PROB vs. planning_problem(PROB) /\ scc_vs(PROB, vs) ==> vs SUBSET FDOM(PROB.I)``,
@@ -1399,7 +1151,7 @@ val scc_main_lemma_1_1_1_2 = store_thm("scc_main_lemma_1_1_1_2",
 METIS_TAC[scc_disjoint_lemma, scc_vs_def])
 
 val scc_main_lemma_1_1_1 = store_thm("scc_main_lemma_1_1_1",
-``!PROB S vs. planning_problem(PROB) /\ FDOM(PROB.I) SUBSET BIGUNION S /\ scc_set(PROB, S) /\ scc_vs(PROB, vs)
+``!PROB S vs. planning_problem(PROB) /\ FDOM(PROB.I) SUBSET BIGUNION S /\ scc_set PROB S /\ scc_vs(PROB, vs)
               ==> vs IN S``,
 SRW_TAC[][]
 THEN `!v. v IN vs ==> ( vs IN S' (* /\ v IN vs' /\ scc_vs(PROB, vs') /\ (vs' = vs)*))` by 
@@ -1420,7 +1172,7 @@ THEN FULL_SIMP_TAC(srw_ss())[scc_vs_def, SCC_def |> Q.SPECL [`(λv1' v2'. dep (P
 THEN METIS_TAC[MEMBER_NOT_EMPTY]);
  
 val scc_main_lemma_1_1 = store_thm("scc_main_lemma_1_1",
-``!PROB S. planning_problem(PROB) /\ FDOM PROB.I SUBSET BIGUNION S /\ scc_set(PROB, S)
+``!PROB S. planning_problem(PROB) /\ FDOM PROB.I SUBSET BIGUNION S /\ scc_set PROB S
            ==> (childless_problem_scc_set(PROB) = member_leaves(PROB, S))``,
 SRW_TAC[][childless_problem_scc_set_def, member_leaves_def, EXTENSION]
 THEN EQ_TAC
@@ -1432,10 +1184,8 @@ val scc_main_lemma_1_2_1 = store_thm("scc_main_lemma_1_2_1",
 SRW_TAC[][]
 THEN SPOSE_NOT_THEN STRIP_ASSUME_TAC
 THEN FULL_SIMP_TAC(bool_ss)[GSYM MEMBER_NOT_EMPTY, scc_vs_def, SCC_def]
-THEN `(λv1' v2'. dep (PROB,v1',v2'))⁺ x x ∧
- (λv1' v2'. dep (PROB,v1',v2'))⁺ x x` by SRW_TAC[][]
-THEN MP_TAC(scc_main_lemma_1_1_1_1_1 |> Q.SPECL [`PROB`, `x`, `x`])
-THEN SRW_TAC[][dep_tc_def])
+THEN FULL_SIMP_TAC(srw_ss())[SUBSET_DEF, EXTENSION]
+THEN METIS_TAC[])
 
 
 val scc_main_lemma_1_2_2_1 = store_thm("scc_main_lemma_1_2_2_1",
@@ -1502,11 +1252,11 @@ THENL
 ])
 
 val scc_main_lemma_1_3 = store_thm("scc_main_lemma_1_3",
-``!PROB S S'. scc_set(PROB, S) /\ S' SUBSET S ==> scc_set(prob_proj(PROB, FDOM(PROB.I) DIFF BIGUNION S'), S)``,
+``!PROB S S'. scc_set PROB S /\ S' SUBSET S ==> scc_set (prob_proj(PROB, FDOM(PROB.I) DIFF BIGUNION S')) S``,
 cheat)
 
 val scc_main_lemma_1_4 = store_thm("scc_main_lemma_1_4",
-``!PROB vs S. scc_set(PROB, S) /\ scc_vs(PROB, vs) /\ FDOM(PROB.I) SUBSET BIGUNION S 
+``!PROB vs S. scc_set PROB S /\ scc_vs(PROB, vs) /\ FDOM(PROB.I) SUBSET BIGUNION S 
               ==> single_child_ancestors PROB vs SUBSET S``,
 cheat)
 
@@ -1533,14 +1283,14 @@ cheat)
 val scc_main_lemma_1 = store_thm("scc_main_lemma_1",
 ``∀s. FINITE s ⇒  
       ∀S PROB.
-       planning_problem PROB ∧ scc_set (PROB,S) ∧
+       planning_problem PROB ∧ scc_set PROB S ∧
        FDOM PROB.I ⊆ BIGUNION S ∧ (S ≠ ∅ ∧ S ≠ {∅}) ∧ FINITE S ∧
        (s = member_leaves (PROB,S)) ⇒
        problem_plan_bound PROB ≤
        sum_scc_parents (PROB,member_leaves (PROB,S))``,
 MATCH_MP_TAC(simpLib.ASM_SIMP_RULE (srw_ss()) [AND_IMP_INTRO]  (FINITE_INDUCT 
    |> INST_TYPE [alpha |-> ``:'a -> bool``] 
-   |> Q.SPEC `(\s. !S PROB. planning_problem PROB ∧ scc_set (PROB,S) 
+   |> Q.SPEC `(\s. !S PROB. planning_problem PROB ∧ scc_set PROB S 
                    ∧ FDOM PROB.I ⊆ BIGUNION S ∧ (BIGUNION S ≠ ∅ ) ∧ FINITE S 
                    /\ (s = member_leaves(PROB, S)) 
                    ==> problem_plan_bound PROB ≤ sum_scc_parents (PROB,s))`))
@@ -1582,34 +1332,6 @@ THENL
    THEN SRW_TAC[][]
    THEN FULL_SIMP_TAC(bool_ss)[((sum_scc_parents_def) |> Q.SPECL [`PROB`, `s`])]
    THEN DECIDE_TAC])
-
-val scc_main_lemma = store_thm("scc_main_lemma",
-``!S PROB. planning_problem(PROB) /\ scc_set(PROB, S) /\ FDOM PROB.I SUBSET BIGUNION S /\ ~(BIGUNION S = EMPTY)
-           /\ FINITE(S)
-           ==>  problem_plan_bound(PROB) <= sum_scc_parents(PROB, (member_leaves(PROB, S)))``,
-NTAC 2 STRIP_TAC 
-THEN MP_TAC(scc_lemma_1_1 |> Q.SPECL [`PROB`, `S'`])
-THEN SRW_TAC[][]
-THEN FULL_SIMP_TAC(srw_ss())[]
-THEN METIS_TAC [scc_main_lemma_1]
-(*
-THEN   Q.UNDISCH_TAC `FINITE (member_leaves (PROB,S'))`
-   THEN Q.UNDISCH_TAC `planning_problem PROB`
-   THEN Q.UNDISCH_TAC `scc_set (PROB,S')`
-   THEN Q.UNDISCH_TAC `FDOM PROB.I ⊆ BIGUNION S'`
-   THEN Q.UNDISCH_TAC `S' ≠ ∅`
-   THEN Q.UNDISCH_TAC `S' ≠ {∅}`
-   THEN Q.UNDISCH_TAC `FINITE S'`
-THEN REWRITE_TAC[AND_IMP_INTRO, GSYM CONJ_ASSOC]
-THEN Q.SPEC_TAC(`S'`, `S'`)
-THEN Q.SPEC_TAC(`PROB`, `PROB`)
-THEN MATCH_MP_TAC(simpLib.ASM_SIMP_RULE (bool_ss) [AND_IMP_INTRO]((CONV_RULE RIGHT_IMP_FORALL_CONV) (simpLib.ASM_SIMP_RULE (srw_ss()) [AND_IMP_INTRO] (GSYM(FINITE_INDUCT 
-   |> INST_TYPE [alpha |-> ``:'a -> bool``] 
-   |> Q.SPEC `(\s. !S PROB. planning_problem PROB ∧ scc_set (PROB,S) 
-                   ∧ FDOM PROB.I ⊆ BIGUNION S ∧ (BIGUNION S ≠ ∅ ) ∧ FINITE S 
-                   /\ (s = member_leaves(PROB, S)) 
-                   ==> problem_plan_bound PROB ≤ sum_scc_parents (PROB,s))`))))) *)
-);
 
 
 val _ = export_theory();
